case type_conv done

theories/BasicAST.v
@@ -6,4 +6,30 @@ Set Primitive Projections.
 Inductive level := 
 | ty (n : nat) | prop.
 
+
+Definition ax (l : level) :=
+  match l with
+  | prop => 0
+  | ty i => S i
+  end.
+
+Definition ru l j :=
+    match l with
+    | prop => j
+    | ty i => max i j
+    end.
+
+
+
+Definition Ax (l : level) : level :=
+  ty (ax l).
+
+Definition Ru (l1 l2 : level) : level :=
+  match l2 with
+  | prop => prop
+  | ty j => ty (ru l1 j)
+  end.
+
+
+
 Definition aref := nat.
