theories/Typing.v
@@ -13,29 +13,6 @@ Set Default Goal Selector "!".
 
 Open Scope subst_scope.
 
-Definition ax (l : level) :=
-  match l with
-  | prop => 0
-  | ty i => S i
-  end.
-
-Definition ru l j :=
-    match l with
-    | prop => j
-    | ty i => max i j
-    end.
-
-
-
-Definition Ax (l : level) : level :=
-  ty (ax l).
-
-Definition Ru (l1 l2 : level) : level :=
-  match l2 with
-  | prop => prop
-  | ty j => ty (ru l1 j)
-  end.
-
 
 Parameter assm_sig : list term.
 
